<?xml version="1.0"?>
<rdf:RDF xmlns="https://www.w3id.org/simulation/ontology/"
     xml:base="https://www.w3id.org/simulation/ontology/"
     xmlns:dc="http://purl.org/dc/elements/1.1/"
     xmlns:owl="http://www.w3.org/2002/07/owl#"
     xmlns:rdf="http://www.w3.org/1999/02/22-rdf-syntax-ns#"
     xmlns:sim="https://www.w3id.org/simulation/ontology/"
     xmlns:xml="http://www.w3.org/XML/1998/namespace"
     xmlns:xsd="http://www.w3.org/2001/XMLSchema#"
     xmlns:rdfs="http://www.w3.org/2000/01/rdf-schema#"
     xmlns:vocab="https://www.w3.org/1999/xhtml/vocab#">
    <owl:Ontology rdf:about="https://www.w3id.org/simulation/ontology/">
        <dc:contributor>Aldo Gangemi</dc:contributor>
        <dc:contributor>Marieke van Erp</dc:contributor>
        <dc:creator>Bruno Sartini</dc:creator>
        <dc:title xml:lang="en">Simulation Ontology</dc:title>
        <rdfs:comment xml:lang="en">This ontology was designed to conceptualize symbolic meanings following Baudrillard&apos;s Simulacra and Simulation theory. Symbols, their meaning, the context in which the symbolic meaning (or simulation) exists and the source of the simulation are linked to a N-ary Simulation Class.</rdfs:comment>
        <rdfs:label xml:lang="en">Simulation Ontology</rdfs:label>
    </owl:Ontology>
    


    <!-- 
    ///////////////////////////////////////////////////////////////////////////////////////
    //
    // Annotation properties
    //
    ///////////////////////////////////////////////////////////////////////////////////////
     -->

    


    <!-- http://purl.org/dc/elements/1.1/contributor -->

    <owl:AnnotationProperty rdf:about="http://purl.org/dc/elements/1.1/contributor"/>
    


    <!-- http://purl.org/dc/elements/1.1/creator -->

    <owl:AnnotationProperty rdf:about="http://purl.org/dc/elements/1.1/creator"/>
    


    <!-- http://purl.org/dc/elements/1.1/license -->

    <owl:AnnotationProperty rdf:about="http://purl.org/dc/elements/1.1/license"/>
    


    <!-- http://purl.org/dc/elements/1.1/title -->

    <owl:AnnotationProperty rdf:about="http://purl.org/dc/elements/1.1/title"/>
    


    <!-- https://www.w3.org/1999/xhtml/vocab#license -->

    <owl:AnnotationProperty rdf:about="https://www.w3.org/1999/xhtml/vocab#license"/>
    


    <!-- 
    ///////////////////////////////////////////////////////////////////////////////////////
    //
    // Object Properties
    //
    ///////////////////////////////////////////////////////////////////////////////////////
     -->

    


    <!-- http://www.w3.org/ns/prov#wasDerivedFrom -->

    <owl:ObjectProperty rdf:about="http://www.w3.org/ns/prov#wasDerivedFrom">
        <rdfs:domain rdf:resource="http://www.w3.org/ns/prov#Entity"/>
        <rdfs:range rdf:resource="http://www.w3.org/ns/prov#Entity"/>
        <rdfs:label>was derived from</rdfs:label>
    </owl:ObjectProperty>
    


    <!-- https://www.w3id.org/simulation/ontology/easedRealityCounterpart -->

    <owl:ObjectProperty rdf:about="https://www.w3id.org/simulation/ontology/easedRealityCounterpart">
        <rdfs:subPropertyOf rdf:resource="https://www.w3id.org/simulation/ontology/hasRealityCounterpart"/>
        <rdfs:domain rdf:resource="https://www.w3id.org/simulation/ontology/Simulation"/>
        <rdfs:range rdf:resource="https://www.w3id.org/simulation/ontology/RealityCounterpart"/>
        <rdfs:comment xml:lang="en">A specific relationship that links a simulation to a reality counterpart that is symbolically eased by the simulacrum. Like the Onyx, which in Indic-Persian context is believed to symbolically ease childbirth.</rdfs:comment>
        <rdfs:isDefinedBy rdf:resource="https://www.w3id.org/simulation/ontology/SimulationOntology"/>
        <rdfs:label xml:lang="en">Eased reality counterpart</rdfs:label>
    </owl:ObjectProperty>
    


    <!-- https://www.w3id.org/simulation/ontology/elicitedRealityCounterpart -->

    <owl:ObjectProperty rdf:about="https://www.w3id.org/simulation/ontology/elicitedRealityCounterpart">
        <rdfs:subPropertyOf rdf:resource="https://www.w3id.org/simulation/ontology/hasRealityCounterpart"/>
        <rdfs:domain rdf:resource="https://www.w3id.org/simulation/ontology/Simulation"/>
        <rdfs:range rdf:resource="https://www.w3id.org/simulation/ontology/RealityCounterpart"/>
        <rdfs:comment xml:lang="en">A specific relationship that links a simulation to a reality counterpart that is symbolically elicited by the simulacrum.</rdfs:comment>
        <rdfs:isDefinedBy rdf:resource="https://www.w3id.org/simulation/ontology/SimulationOntology"/>
        <rdfs:label xml:lang="en">Elicited reality counterpart</rdfs:label>
    </owl:ObjectProperty>
    


    <!-- https://www.w3id.org/simulation/ontology/hasContext -->

    <owl:ObjectProperty rdf:about="https://www.w3id.org/simulation/ontology/hasContext">
        <owl:inverseOf rdf:resource="https://www.w3id.org/simulation/ontology/isContextOf"/>
        <rdfs:domain rdf:resource="https://www.w3id.org/simulation/ontology/Simulation"/>
        <rdfs:range rdf:resource="https://www.w3id.org/simulation/ontology/Context"/>
        <rdfs:comment xml:lang="en">This property links a Simulation to its context</rdfs:comment>
        <rdfs:isDefinedBy rdf:resource="https://www.w3id.org/simulation/ontology/SimulationOntology"/>
        <rdfs:label xml:lang="en">has Context</rdfs:label>
    </owl:ObjectProperty>
    


    <!-- https://www.w3id.org/simulation/ontology/hasPersonifiedVariant -->

    <owl:ObjectProperty rdf:about="https://www.w3id.org/simulation/ontology/hasPersonifiedVariant">
        <rdfs:subPropertyOf rdf:resource="https://www.w3id.org/simulation/ontology/hasVariant"/>
        <owl:inverseOf rdf:resource="https://www.w3id.org/simulation/ontology/isPersonifiedVariantOf"/>
        <rdfs:domain>
            <owl:Class>
                <owl:unionOf rdf:parseType="Collection">
                    <rdf:Description rdf:about="https://www.w3id.org/simulation/ontology/RealityCounterpart"/>
                    <rdf:Description rdf:about="https://www.w3id.org/simulation/ontology/Simulacrum"/>
                </owl:unionOf>
            </owl:Class>
        </rdfs:domain>
        <rdfs:range>
            <owl:Class>
                <owl:unionOf rdf:parseType="Collection">
                    <rdf:Description rdf:about="https://www.w3id.org/simulation/ontology/RealityCounterpart"/>
                    <rdf:Description rdf:about="https://www.w3id.org/simulation/ontology/Simulacrum"/>
                </owl:unionOf>
            </owl:Class>
        </rdfs:range>
        <rdfs:comment xml:lang="en">This property is used when a variant is intended as the personified variant of the other entity. Like &quot;Air&quot; has personified variant &quot;Air personified&quot;</rdfs:comment>
        <rdfs:isDefinedBy rdf:resource="https://www.w3id.org/simulation/ontology/SimulationOntology"/>
        <rdfs:label xml:lang="en">Has personified variant</rdfs:label>
    </owl:ObjectProperty>
    


    <!-- https://www.w3id.org/simulation/ontology/hasRealityCounterpart -->

    <owl:ObjectProperty rdf:about="https://www.w3id.org/simulation/ontology/hasRealityCounterpart">
        <owl:inverseOf rdf:resource="https://www.w3id.org/simulation/ontology/isRealityCounterpartOf"/>
        <rdfs:domain rdf:resource="https://www.w3id.org/simulation/ontology/Simulation"/>
        <rdfs:range rdf:resource="https://www.w3id.org/simulation/ontology/RealityCounterpart"/>
        <rdfs:comment xml:lang="en">This property links a Simulation to its reality counterpart. More specific relationships between a simulation and its reality counterpart are available as subproperties of this property.</rdfs:comment>
        <rdfs:isDefinedBy rdf:resource="https://www.w3id.org/simulation/ontology/SimulationOntology"/>
        <rdfs:label xml:lang="en">Has reality counterpart</rdfs:label>
    </owl:ObjectProperty>
    


    <!-- https://www.w3id.org/simulation/ontology/hasSimulacrum -->

    <owl:ObjectProperty rdf:about="https://www.w3id.org/simulation/ontology/hasSimulacrum">
        <owl:inverseOf rdf:resource="https://www.w3id.org/simulation/ontology/isSimulacrumOf"/>
        <rdf:type rdf:resource="http://www.w3.org/2002/07/owl#FunctionalProperty"/>
        <rdfs:domain rdf:resource="https://www.w3id.org/simulation/ontology/Simulation"/>
        <rdfs:range rdf:resource="https://www.w3id.org/simulation/ontology/Simulacrum"/>
        <rdfs:comment xml:lang="en">This property links a simulation to its simulacrum.</rdfs:comment>
        <rdfs:isDefinedBy rdf:resource="https://www.w3id.org/simulation/ontology/SimulationOntology"/>
        <rdfs:label xml:lang="en">Has simulacrum</rdfs:label>
    </owl:ObjectProperty>
    


    <!-- https://www.w3id.org/simulation/ontology/hasSource -->

    <owl:ObjectProperty rdf:about="https://www.w3id.org/simulation/ontology/hasSource">
        <rdfs:subPropertyOf rdf:resource="http://www.w3.org/ns/prov#wasDerivedFrom"/>
        <owl:inverseOf rdf:resource="https://www.w3id.org/simulation/ontology/isSourceOf"/>
        <rdfs:domain rdf:resource="https://www.w3id.org/simulation/ontology/Simulation"/>
        <rdfs:range rdf:resource="https://www.w3id.org/simulation/ontology/Source"/>
        <rdfs:comment xml:lang="en">This property links a Simulation with its source</rdfs:comment>
        <rdfs:isDefinedBy rdf:resource="https://www.w3id.org/simulation/ontology/SimulationOntology"/>
        <rdfs:label xml:lang="en">Has source</rdfs:label>
    </owl:ObjectProperty>
    


    <!-- https://www.w3id.org/simulation/ontology/hasVariant -->

    <owl:ObjectProperty rdf:about="https://www.w3id.org/simulation/ontology/hasVariant">
        <owl:inverseOf rdf:resource="https://www.w3id.org/simulation/ontology/isVariantOf"/>
        <rdfs:domain>
            <owl:Class>
                <owl:unionOf rdf:parseType="Collection">
                    <rdf:Description rdf:about="https://www.w3id.org/simulation/ontology/RealityCounterpart"/>
                    <rdf:Description rdf:about="https://www.w3id.org/simulation/ontology/Simulacrum"/>
                </owl:unionOf>
            </owl:Class>
        </rdfs:domain>
        <rdfs:range>
            <owl:Class>
                <owl:unionOf rdf:parseType="Collection">
                    <rdf:Description rdf:about="https://www.w3id.org/simulation/ontology/RealityCounterpart"/>
                    <rdf:Description rdf:about="https://www.w3id.org/simulation/ontology/Simulacrum"/>
                </owl:unionOf>
            </owl:Class>
        </rdfs:range>
        <rdfs:comment xml:lang="en">This property links a simulacrum or a reality counterpart to a variant of theirs. A variant is intended as a narrower concept than one of those two elements. It is also used to define a set of elements in relation to a single element that is part of that set. I.e. &quot;man and woman&quot; is a variant of &quot;woman&quot;, &quot;golden apple&quot; is a variant of &quot;apple&quot;.</rdfs:comment>
        <rdfs:isDefinedBy rdf:resource="https://www.w3id.org/simulation/ontology/SimulationOntology"/>
        <rdfs:label xml:lang="en">has variant</rdfs:label>
    </owl:ObjectProperty>
    


    <!-- https://www.w3id.org/simulation/ontology/healedRealityCounterpart -->

    <owl:ObjectProperty rdf:about="https://www.w3id.org/simulation/ontology/healedRealityCounterpart">
        <rdfs:subPropertyOf rdf:resource="https://www.w3id.org/simulation/ontology/hasRealityCounterpart"/>
        <rdfs:domain rdf:resource="https://www.w3id.org/simulation/ontology/HealingSimulation"/>
        <rdfs:range rdf:resource="https://www.w3id.org/simulation/ontology/RealityCounterpart"/>
        <rdfs:comment xml:lang="en">A specific relationship that links a simulation (usually a Healing Simulation) to a reality counterpart of which a simulacrum is the symbolic cure.</rdfs:comment>
        <rdfs:isDefinedBy rdf:resource="https://www.w3id.org/simulation/ontology/SimulationOntology"/>
        <rdfs:label xml:lang="en">Healed reality counterpart</rdfs:label>
    </owl:ObjectProperty>
    


    <!-- https://www.w3id.org/simulation/ontology/isContextOf -->

    <owl:ObjectProperty rdf:about="https://www.w3id.org/simulation/ontology/isContextOf">
        <rdfs:domain rdf:resource="https://www.w3id.org/simulation/ontology/Context"/>
        <rdfs:range rdf:resource="https://www.w3id.org/simulation/ontology/Simulation"/>
        <rdfs:comment xml:lang="en">inverse property of has context</rdfs:comment>
        <rdfs:isDefinedBy rdf:resource="https://www.w3id.org/simulation/ontology/SimulationOntology"/>
        <rdfs:label xml:lang="en">Is context of</rdfs:label>
    </owl:ObjectProperty>
    


    <!-- https://www.w3id.org/simulation/ontology/isEasedRealityCounterpartOf -->

    <owl:ObjectProperty rdf:about="https://www.w3id.org/simulation/ontology/isEasedRealityCounterpartOf">
        <rdfs:subPropertyOf rdf:resource="https://www.w3id.org/simulation/ontology/isRealityCounterpartOf"/>
        <rdfs:domain rdf:resource="https://www.w3id.org/simulation/ontology/RealityCounterpart"/>
        <rdfs:range rdf:resource="https://www.w3id.org/simulation/ontology/Simulation"/>
        <rdfs:comment xml:lang="en">Inverse property of eased reality counterpart</rdfs:comment>
        <rdfs:isDefinedBy rdf:resource="https://www.w3id.org/simulation/ontology/SimulationOntology"/>
        <rdfs:label xml:lang="en">Is eased reality counterpart of</rdfs:label>
    </owl:ObjectProperty>
    


    <!-- https://www.w3id.org/simulation/ontology/isElicitedRealityCounterpartOf -->

    <owl:ObjectProperty rdf:about="https://www.w3id.org/simulation/ontology/isElicitedRealityCounterpartOf">
        <rdfs:subPropertyOf rdf:resource="https://www.w3id.org/simulation/ontology/isRealityCounterpartOf"/>
        <rdfs:domain rdf:resource="https://www.w3id.org/simulation/ontology/RealityCounterpart"/>
        <rdfs:range rdf:resource="https://www.w3id.org/simulation/ontology/Simulation"/>
        <rdfs:comment xml:lang="en">Inverse property of elicited reality counterpart</rdfs:comment>
        <rdfs:isDefinedBy rdf:resource="https://www.w3id.org/simulation/ontology/SimulationOntology"/>
        <rdfs:label xml:lang="en">Is elicited reality counterpart of</rdfs:label>
    </owl:ObjectProperty>
    


    <!-- https://www.w3id.org/simulation/ontology/isHealedRealityCounterpartOf -->

    <owl:ObjectProperty rdf:about="https://www.w3id.org/simulation/ontology/isHealedRealityCounterpartOf">
        <rdfs:subPropertyOf rdf:resource="https://www.w3id.org/simulation/ontology/isRealityCounterpartOf"/>
        <rdfs:domain rdf:resource="https://www.w3id.org/simulation/ontology/RealityCounterpart"/>
        <rdfs:range rdf:resource="https://www.w3id.org/simulation/ontology/HealingSimulation"/>
        <rdfs:comment xml:lang="en">Inverse property of healed reality counterpart</rdfs:comment>
        <rdfs:isDefinedBy rdf:resource="https://www.w3id.org/simulation/ontology/SimulationOntology"/>
        <rdfs:label xml:lang="en">Is healed reality counterpart of</rdfs:label>
    </owl:ObjectProperty>
    


    <!-- https://www.w3id.org/simulation/ontology/isPersonifiedVariantOf -->

    <owl:ObjectProperty rdf:about="https://www.w3id.org/simulation/ontology/isPersonifiedVariantOf">
        <rdfs:subPropertyOf rdf:resource="https://www.w3id.org/simulation/ontology/isVariantOf"/>
        <rdfs:domain>
            <owl:Class>
                <owl:unionOf rdf:parseType="Collection">
                    <rdf:Description rdf:about="https://www.w3id.org/simulation/ontology/RealityCounterpart"/>
                    <rdf:Description rdf:about="https://www.w3id.org/simulation/ontology/Simulacrum"/>
                </owl:unionOf>
            </owl:Class>
        </rdfs:domain>
        <rdfs:range>
            <owl:Class>
                <owl:unionOf rdf:parseType="Collection">
                    <rdf:Description rdf:about="https://www.w3id.org/simulation/ontology/RealityCounterpart"/>
                    <rdf:Description rdf:about="https://www.w3id.org/simulation/ontology/Simulacrum"/>
                </owl:unionOf>
            </owl:Class>
        </rdfs:range>
        <rdfs:comment xml:lang="en">Inverse property of has personified variant</rdfs:comment>
        <rdfs:isDefinedBy rdf:resource="https://www.w3id.org/simulation/ontology/SimulationOntology"/>
        <rdfs:label xml:lang="en">Is personified variant of</rdfs:label>
    </owl:ObjectProperty>
    


    <!-- https://www.w3id.org/simulation/ontology/isPreventedRealityCounterpartOf -->

    <owl:ObjectProperty rdf:about="https://www.w3id.org/simulation/ontology/isPreventedRealityCounterpartOf">
        <rdfs:subPropertyOf rdf:resource="https://www.w3id.org/simulation/ontology/isRealityCounterpartOf"/>
        <rdfs:domain rdf:resource="https://www.w3id.org/simulation/ontology/RealityCounterpart"/>
        <rdfs:range rdf:resource="https://www.w3id.org/simulation/ontology/ProtectionSimulation"/>
        <rdfs:comment xml:lang="en">Inversed property of prevented reality counterpart</rdfs:comment>
        <rdfs:isDefinedBy rdf:resource="https://www.w3id.org/simulation/ontology/SimulationOntology"/>
        <rdfs:label xml:lang="en">Is prevented reality counterpart of</rdfs:label>
    </owl:ObjectProperty>
    


    <!-- https://www.w3id.org/simulation/ontology/isRealityCounterpartOf -->

    <owl:ObjectProperty rdf:about="https://www.w3id.org/simulation/ontology/isRealityCounterpartOf">
        <rdfs:domain rdf:resource="https://www.w3id.org/simulation/ontology/RealityCounterpart"/>
        <rdfs:range rdf:resource="https://www.w3id.org/simulation/ontology/Simulation"/>
        <rdfs:comment xml:lang="en">Inversed property of has reality counterpart</rdfs:comment>
        <rdfs:isDefinedBy rdf:resource="https://www.w3id.org/simulation/ontology/SimulationOntology"/>
        <rdfs:label xml:lang="en">Is reality counterpart of</rdfs:label>
    </owl:ObjectProperty>
    


    <!-- https://www.w3id.org/simulation/ontology/isRestoredRealityCounterpartOf -->

    <owl:ObjectProperty rdf:about="https://www.w3id.org/simulation/ontology/isRestoredRealityCounterpartOf">
        <rdfs:subPropertyOf rdf:resource="https://www.w3id.org/simulation/ontology/isRealityCounterpartOf"/>
        <rdfs:domain rdf:resource="https://www.w3id.org/simulation/ontology/RealityCounterpart"/>
        <rdfs:range rdf:resource="https://www.w3id.org/simulation/ontology/ProtectionSimulation"/>
        <rdfs:comment xml:lang="en">Inverse property of restored reality counterpart</rdfs:comment>
        <rdfs:isDefinedBy rdf:resource="https://www.w3id.org/simulation/ontology/SimulationOntology"/>
        <rdfs:label xml:lang="en">Is restored reality counterpart of</rdfs:label>
    </owl:ObjectProperty>
    


    <!-- https://www.w3id.org/simulation/ontology/isSimulacrumOf -->

    <owl:ObjectProperty rdf:about="https://www.w3id.org/simulation/ontology/isSimulacrumOf">
        <rdfs:domain rdf:resource="https://www.w3id.org/simulation/ontology/Simulacrum"/>
        <rdfs:range rdf:resource="https://www.w3id.org/simulation/ontology/Simulation"/>
        <rdfs:comment xml:lang="en">Inversed property of has simulacrum</rdfs:comment>
        <rdfs:isDefinedBy rdf:resource="https://www.w3id.org/simulation/ontology/SimulationOntology"/>
        <rdfs:label xml:lang="en">Is simulacrum of</rdfs:label>
    </owl:ObjectProperty>
    


    <!-- https://www.w3id.org/simulation/ontology/isSourceOf -->

    <owl:ObjectProperty rdf:about="https://www.w3id.org/simulation/ontology/isSourceOf">
        <rdfs:subPropertyOf>
            <rdf:Description>
                <owl:inverseOf rdf:resource="http://www.w3.org/ns/prov#wasDerivedFrom"/>
            </rdf:Description>
        </rdfs:subPropertyOf>
        <rdfs:domain rdf:resource="https://www.w3id.org/simulation/ontology/Source"/>
        <rdfs:range rdf:resource="https://www.w3id.org/simulation/ontology/Simulation"/>
        <rdfs:comment xml:lang="en">Inverse property of has source</rdfs:comment>
        <rdfs:isDefinedBy rdf:resource="https://www.w3id.org/simulation/ontology/SimulationOntology"/>
        <rdfs:label xml:lang="en">Is source of</rdfs:label>
    </owl:ObjectProperty>
    


    <!-- https://www.w3id.org/simulation/ontology/isVariantOf -->

    <owl:ObjectProperty rdf:about="https://www.w3id.org/simulation/ontology/isVariantOf">
        <rdfs:domain rdf:resource="https://www.w3id.org/simulation/ontology/Simulacrum"/>
        <rdfs:range rdf:resource="https://www.w3id.org/simulation/ontology/Simulacrum"/>
        <rdfs:comment xml:lang="en">Inverse property of has variant</rdfs:comment>
        <rdfs:isDefinedBy rdf:resource="https://www.w3id.org/simulation/ontology/SimulationOntology"/>
        <rdfs:label xml:lang="en">Is variant of</rdfs:label>
    </owl:ObjectProperty>
    


    <!-- https://www.w3id.org/simulation/ontology/preventedRealityCounterpart -->

    <owl:ObjectProperty rdf:about="https://www.w3id.org/simulation/ontology/preventedRealityCounterpart">
        <rdfs:subPropertyOf rdf:resource="https://www.w3id.org/simulation/ontology/hasRealityCounterpart"/>
        <rdfs:domain rdf:resource="https://www.w3id.org/simulation/ontology/ProtectionSimulation"/>
        <rdfs:range rdf:resource="https://www.w3id.org/simulation/ontology/RealityCounterpart"/>
        <rdfs:comment xml:lang="en">A specific relationship that links a simulation (usually a Protection Simulation) to a reality counterpart that is symbolically prevented by the simulacrum.</rdfs:comment>
        <rdfs:isDefinedBy rdf:resource="https://www.w3id.org/simulation/ontology/SimulationOntology"/>
        <rdfs:label xml:lang="en">Prevented reality counterpart</rdfs:label>
    </owl:ObjectProperty>
    


    <!-- https://www.w3id.org/simulation/ontology/restoredRealityCounterpart -->

    <owl:ObjectProperty rdf:about="https://www.w3id.org/simulation/ontology/restoredRealityCounterpart">
        <rdfs:subPropertyOf rdf:resource="https://www.w3id.org/simulation/ontology/hasRealityCounterpart"/>
        <rdfs:domain rdf:resource="https://www.w3id.org/simulation/ontology/Simulation"/>
        <rdfs:range rdf:resource="https://www.w3id.org/simulation/ontology/RealityCounterpart"/>
        <rdfs:comment xml:lang="en">A specific relationship that links a simulation to a reality counterpart that is symbolically restored by the simulacrum. Like the red valerian (simulacrum), which, in flower language, is symbolically believed to restore strenght (restored reality counterpart).</rdfs:comment>
        <rdfs:isDefinedBy rdf:resource="https://www.w3id.org/simulation/ontology/SimulationOntology"/>
        <rdfs:label xml:lang="en">Restored reality counterpart</rdfs:label>
    </owl:ObjectProperty>
    


    <!-- https://www.w3id.org/simulation/ontology/symbolicMeaning -->

    <owl:ObjectProperty rdf:about="https://www.w3id.org/simulation/ontology/symbolicMeaning">
        <rdfs:domain rdf:resource="https://www.w3id.org/simulation/ontology/Simulacrum"/>
        <rdfs:range rdf:resource="https://www.w3id.org/simulation/ontology/RealityCounterpart"/>
        <owl:propertyChainAxiom rdf:parseType="Collection">
            <rdf:Description rdf:about="https://www.w3id.org/simulation/ontology/isSimulacrumOf"/>
            <rdf:Description rdf:about="https://www.w3id.org/simulation/ontology/hasRealityCounterpart"/>
        </owl:propertyChainAxiom>
        <rdfs:comment xml:lang="en">This property is a chain property that links a simulacrum with its reality counterpart. This direct relationship does not consider neither the context or the source of the simulation</rdfs:comment>
        <rdfs:isDefinedBy rdf:resource="https://www.w3id.org/simulation/ontology/SimulationOntology"/>
        <rdfs:label xml:lang="en">Symbolic Meaning</rdfs:label>
    </owl:ObjectProperty>
    


    <!-- 
    ///////////////////////////////////////////////////////////////////////////////////////
    //
    // Classes
    //
    ///////////////////////////////////////////////////////////////////////////////////////
     -->

    


    <!-- http://www.w3.org/ns/prov#Entity -->

    <owl:Class rdf:about="http://www.w3.org/ns/prov#Entity">
        <rdfs:label>Entity</rdfs:label>
    </owl:Class>
    


    <!-- https://www.w3id.org/simulation/ontology/AllusionSimulation -->

    <owl:Class rdf:about="https://www.w3id.org/simulation/ontology/AllusionSimulation">
        <rdfs:subClassOf rdf:resource="https://www.w3id.org/simulation/ontology/Simulation"/>
        <rdfs:comment xml:lang="en">A specific kind of simulation in which the simulacrum alludes to the reality counterpart. Is a more subtle symbolic relationship than the normal simulation.</rdfs:comment>
        <rdfs:label xml:lang="en">Allusion Simulation</rdfs:label>
    </owl:Class>
    


    <!-- https://www.w3id.org/simulation/ontology/AssociationSimulation -->

    <owl:Class rdf:about="https://www.w3id.org/simulation/ontology/AssociationSimulation">
        <rdfs:subClassOf rdf:resource="https://www.w3id.org/simulation/ontology/Simulation"/>
        <rdfs:comment xml:lang="en">A simulation in which the simulacrum is associated with the reality counterpart. It is a very general relationship and should be used only when the association is explicitly stated by the source. I.E. in a dictionary of symbols it is written that X &quot;is associated with&quot; Y.</rdfs:comment>
        <rdfs:isDefinedBy rdf:resource="https://www.w3id.org/simulation/ontology/SimulationOntology"/>
        <rdfs:label xml:lang="en">Association Simulation</rdfs:label>
    </owl:Class>
    


    <!-- https://www.w3id.org/simulation/ontology/AttributeSimulation -->

    <owl:Class rdf:about="https://www.w3id.org/simulation/ontology/AttributeSimulation">
        <rdfs:subClassOf rdf:resource="https://www.w3id.org/simulation/ontology/Simulation"/>
        <rdfs:comment xml:lang="en">A specific kind of simulation in which the simulacrum is a symbolic attribute of the reality counterpart. Like &quot;keys&quot; as an attribute of Saint Peter.</rdfs:comment>
        <rdfs:isDefinedBy rdf:resource="https://www.w3id.org/simulation/ontology/SimulationOntology"/>
        <rdfs:label xml:lang="en">Attribute Simulation</rdfs:label>
    </owl:Class>
    


    <!-- https://www.w3id.org/simulation/ontology/Context -->

    <owl:Class rdf:about="https://www.w3id.org/simulation/ontology/Context">
        <rdfs:subClassOf>
            <owl:Restriction>
                <owl:onProperty rdf:resource="https://www.w3id.org/simulation/ontology/isContextOf"/>
                <owl:someValuesFrom rdf:resource="https://www.w3id.org/simulation/ontology/Simulation"/>
            </owl:Restriction>
        </rdfs:subClassOf>
        <owl:disjointWith rdf:resource="https://www.w3id.org/simulation/ontology/Simulation"/>
        <owl:disjointWith rdf:resource="https://www.w3id.org/simulation/ontology/Source"/>
        <rdfs:comment xml:lang="en">The context is the setting (either social, historical, cultural etc...) in which a Simulation exists. An ash tree, in the Norse context is a symbol of Odin. On the other hand, a tree in a Celtic context is a symbol of connection.</rdfs:comment>
        <rdfs:isDefinedBy rdf:resource="https://www.w3id.org/simulation/ontology/SimulationOntology"/>
        <rdfs:label xml:lang="en">Context</rdfs:label>
    </owl:Class>
    


    <!-- https://www.w3id.org/simulation/ontology/CorrespondenceSimulation -->

    <owl:Class rdf:about="https://www.w3id.org/simulation/ontology/CorrespondenceSimulation">
        <rdfs:subClassOf rdf:resource="https://www.w3id.org/simulation/ontology/Simulation"/>
        <rdfs:comment xml:lang="en">A simulation in which the simulacrum corresponds to the reality counterpart. It is a very general relationship and should be used only when the correspondence is explicitly state by the source. I.E. in a dictionary of symbols it is written that X &quot;corresponds to&quot; Y.</rdfs:comment>
        <rdfs:isDefinedBy rdf:resource="https://www.w3id.org/simulation/ontology/SimulationOntology"/>
        <rdfs:label xml:lang="en">Correspondence Simulation</rdfs:label>
    </owl:Class>
    


    <!-- https://www.w3id.org/simulation/ontology/EmblematicSimulation -->

    <owl:Class rdf:about="https://www.w3id.org/simulation/ontology/EmblematicSimulation">
        <rdfs:subClassOf rdf:resource="https://www.w3id.org/simulation/ontology/Simulation"/>
        <rdfs:comment xml:lang="en">A specific kind of simulation in which the simulacrum is an emblem of the reality counterpart. Emblems are usually used as a graphical representation of something.</rdfs:comment>
        <rdfs:isDefinedBy rdf:resource="https://www.w3id.org/simulation/ontology/SimulationOntology"/>
        <rdfs:label xml:lang="en">Emblematic Simulation</rdfs:label>
    </owl:Class>
    


    <!-- https://www.w3id.org/simulation/ontology/HealingSimulation -->

    <owl:Class rdf:about="https://www.w3id.org/simulation/ontology/HealingSimulation">
        <rdfs:subClassOf rdf:resource="https://www.w3id.org/simulation/ontology/Simulation"/>
        <rdfs:subClassOf>
            <owl:Restriction>
                <owl:onProperty rdf:resource="https://www.w3id.org/simulation/ontology/healedRealityCounterpart"/>
                <owl:qualifiedCardinality rdf:datatype="http://www.w3.org/2001/XMLSchema#nonNegativeInteger">1</owl:qualifiedCardinality>
                <owl:onClass rdf:resource="https://www.w3id.org/simulation/ontology/RealityCounterpart"/>
            </owl:Restriction>
        </rdfs:subClassOf>
        <owl:hasKey rdf:parseType="Collection">
            <rdf:Description rdf:about="https://www.w3id.org/simulation/ontology/hasSimulacrum"/>
            <rdf:Description rdf:about="https://www.w3id.org/simulation/ontology/healedRealityCounterpart"/>
        </owl:hasKey>
        <rdfs:comment xml:lang="en">A specific kind of simulation in which the simulacrum is a symbolic cure for the reality counterpart. The reality counterpart in this kind of simulation is in fact usually something negative like a disease or a curse.</rdfs:comment>
        <rdfs:isDefinedBy rdf:resource="https://www.w3id.org/simulation/ontology/SimulationOntology"/>
        <rdfs:label xml:lang="en">Healing Simulation</rdfs:label>
    </owl:Class>
    


    <!-- https://www.w3id.org/simulation/ontology/ManifestationSimulation -->

    <owl:Class rdf:about="https://www.w3id.org/simulation/ontology/ManifestationSimulation">
        <rdfs:subClassOf rdf:resource="https://www.w3id.org/simulation/ontology/Simulation"/>
        <rdfs:comment xml:lang="en">A simulation in which the simulacrum is a manifestation of the reality counterpart. It is a very general relationship and should be used only when the manifestation is explicitly stated by the source. I.E. in a dictionary of symbols it is written than X &quot;is a manifestation of&quot; Y.</rdfs:comment>
        <rdfs:isDefinedBy rdf:resource="https://www.w3id.org/simulation/ontology/SimulationOntology"/>
        <rdfs:label xml:lang="en">Manifestation Simulation</rdfs:label>
    </owl:Class>
    


    <!-- https://www.w3id.org/simulation/ontology/ProtectionSimulation -->

    <owl:Class rdf:about="https://www.w3id.org/simulation/ontology/ProtectionSimulation">
        <rdfs:subClassOf rdf:resource="https://www.w3id.org/simulation/ontology/Simulation"/>
        <rdfs:subClassOf>
            <owl:Restriction>
                <owl:onProperty rdf:resource="https://www.w3id.org/simulation/ontology/preventedRealityCounterpart"/>
                <owl:qualifiedCardinality rdf:datatype="http://www.w3.org/2001/XMLSchema#nonNegativeInteger">1</owl:qualifiedCardinality>
                <owl:onClass rdf:resource="https://www.w3id.org/simulation/ontology/RealityCounterpart"/>
            </owl:Restriction>
        </rdfs:subClassOf>
        <owl:hasKey rdf:parseType="Collection">
            <rdf:Description rdf:about="https://www.w3id.org/simulation/ontology/hasSimulacrum"/>
            <rdf:Description rdf:about="https://www.w3id.org/simulation/ontology/preventedRealityCounterpart"/>
        </owl:hasKey>
        <rdfs:comment xml:lang="en">A specific kind of simulation in which the simulacrum is a symbolic protection against the reality counterpart. Like agate as a protection against the evil eye.</rdfs:comment>
        <rdfs:isDefinedBy rdf:resource="https://www.w3id.org/simulation/ontology/SimulationOntology"/>
        <rdfs:label xml:lang="en">Protection Simulation</rdfs:label>
    </owl:Class>
    


    <!-- https://www.w3id.org/simulation/ontology/RealityCounterpart -->

    <owl:Class rdf:about="https://www.w3id.org/simulation/ontology/RealityCounterpart">
        <rdfs:subClassOf>
            <owl:Restriction>
                <owl:onProperty rdf:resource="https://www.w3id.org/simulation/ontology/isRealityCounterpartOf"/>
                <owl:someValuesFrom rdf:resource="https://www.w3id.org/simulation/ontology/Simulation"/>
            </owl:Restriction>
        </rdfs:subClassOf>
        <rdfs:comment xml:lang="en">A reality counterpart is the symbolic meaning associated to a simulacrum. It&apos;s the element that is symbolically referred by the simulacrum in a simulation. The term is taken from Baudrillard&apos;s Simulacra and Simulation theory</rdfs:comment>
        <rdfs:isDefinedBy rdf:resource="https://www.w3id.org/simulation/ontology/SimulationOntology"/>
        <rdfs:label xml:lang="en">Reality Counterpart</rdfs:label>
    </owl:Class>
    


    <!-- https://www.w3id.org/simulation/ontology/RelatednessSimulation -->

    <owl:Class rdf:about="https://www.w3id.org/simulation/ontology/RelatednessSimulation">
        <rdfs:subClassOf rdf:resource="https://www.w3id.org/simulation/ontology/Simulation"/>
        <rdfs:comment xml:lang="en">A simulation in which the simulacrum is related to the reality counterpart. It is a very general relationship and should be used only when the relatedness is explicitly stated by the source. I.E. in a dictionary of symbols it is written that X &quot;is related to&quot; Y.</rdfs:comment>
        <rdfs:isDefinedBy rdf:resource="https://www.w3id.org/simulation/ontology/SimulationOntology"/>
        <rdfs:label xml:lang="en">Relatedness Simulation</rdfs:label>
    </owl:Class>
    


    <!-- https://www.w3id.org/simulation/ontology/Simulacrum -->

    <owl:Class rdf:about="https://www.w3id.org/simulation/ontology/Simulacrum">
        <rdfs:subClassOf>
            <owl:Restriction>
                <owl:onProperty rdf:resource="https://www.w3id.org/simulation/ontology/isSimulacrumOf"/>
                <owl:someValuesFrom rdf:resource="https://www.w3id.org/simulation/ontology/Simulation"/>
            </owl:Restriction>
        </rdfs:subClassOf>
        <rdfs:comment xml:lang="en">A simulacrum is something that carries a secondary meaning (the first being its literal meaning), of symbolic nature. i.e. a skull is the set of bones of a head (literal meaning), but it is also the symbol of death (secondary, symbolic meaning). The term is taken from Baudrillard&apos;s Simulacra and Simulation theory. The plural of simulacrum is simulacra.</rdfs:comment>
        <rdfs:isDefinedBy rdf:resource="https://www.w3id.org/simulation/ontology/SimulationOntology"/>
        <rdfs:label xml:lang="en">Simulacrum</rdfs:label>
    </owl:Class>
    


    <!-- https://www.w3id.org/simulation/ontology/Simulation -->

    <owl:Class rdf:about="https://www.w3id.org/simulation/ontology/Simulation">
        <rdfs:subClassOf>
            <owl:Restriction>
                <owl:onProperty rdf:resource="https://www.w3id.org/simulation/ontology/hasContext"/>
                <owl:someValuesFrom rdf:resource="https://www.w3id.org/simulation/ontology/Context"/>
            </owl:Restriction>
        </rdfs:subClassOf>
        <rdfs:subClassOf>
            <owl:Restriction>
                <owl:onProperty rdf:resource="https://www.w3id.org/simulation/ontology/hasRealityCounterpart"/>
                <owl:someValuesFrom rdf:resource="https://www.w3id.org/simulation/ontology/RealityCounterpart"/>
            </owl:Restriction>
        </rdfs:subClassOf>
        <rdfs:subClassOf>
            <owl:Restriction>
                <owl:onProperty rdf:resource="https://www.w3id.org/simulation/ontology/hasSource"/>
                <owl:someValuesFrom rdf:resource="https://www.w3id.org/simulation/ontology/Source"/>
            </owl:Restriction>
        </rdfs:subClassOf>
        <rdfs:subClassOf>
            <owl:Restriction>
                <owl:onProperty rdf:resource="https://www.w3id.org/simulation/ontology/hasSimulacrum"/>
                <owl:qualifiedCardinality rdf:datatype="http://www.w3.org/2001/XMLSchema#nonNegativeInteger">1</owl:qualifiedCardinality>
                <owl:onClass rdf:resource="https://www.w3id.org/simulation/ontology/Simulacrum"/>
            </owl:Restriction>
        </rdfs:subClassOf>
        <owl:disjointWith rdf:resource="https://www.w3id.org/simulation/ontology/Source"/>
        <owl:hasKey rdf:parseType="Collection">
            <rdf:Description rdf:about="https://www.w3id.org/simulation/ontology/hasRealityCounterpart"/>
            <rdf:Description rdf:about="https://www.w3id.org/simulation/ontology/hasSimulacrum"/>
        </owl:hasKey>
        <rdfs:comment xml:lang="en">A simulation is the symbolic relationship that happens between a symbol and its symbolic meaning. The term is taken from Baudrillard&apos;s Simulacra and Simulation philosophical theory.</rdfs:comment>
        <rdfs:isDefinedBy rdf:resource="https://www.w3id.org/simulation/ontology/SimulationOntology"/>
        <rdfs:label xml:lang="en">Simulation</rdfs:label>
    </owl:Class>
    


    <!-- https://www.w3id.org/simulation/ontology/Source -->

    <owl:Class rdf:about="https://www.w3id.org/simulation/ontology/Source">
        <rdfs:subClassOf>
            <owl:Restriction>
                <owl:onProperty rdf:resource="https://www.w3id.org/simulation/ontology/isSourceOf"/>
                <owl:someValuesFrom rdf:resource="https://www.w3id.org/simulation/ontology/Simulation"/>
            </owl:Restriction>
        </rdfs:subClassOf>
        <rdfs:comment xml:lang="en">This class represents the source of a simulation. It is intended as the entity that acknowledges a simulation as a legitimate symbolic relationship. A source can either be a dictionary of symbols or a knowledge graph in which symbolic information are present.</rdfs:comment>
        <rdfs:isDefinedBy rdf:resource="https://www.w3id.org/simulation/ontology/SimulationOntology"/>
        <rdfs:label xml:lang="en">Source</rdfs:label>
    </owl:Class>
    


    <!-- 
    ///////////////////////////////////////////////////////////////////////////////////////
    //
    // Individuals
    //
    ///////////////////////////////////////////////////////////////////////////////////////
     -->

    


    <!-- https://www.w3id.org/simulation/ontology/SimulationOntology -->

    <owl:NamedIndividual rdf:about="https://www.w3id.org/simulation/ontology/SimulationOntology"/>
</rdf:RDF>



<!-- Generated by the OWL API (version 4.5.9.2019-02-01T07:24:44Z) https://github.com/owlcs/owlapi -->

